Implement mlswg/mls-protocol#527 + mlswg/mls-protocol#635 (stronger parent-hash)

fstar/MLS.TreeSync.ParentHash.fst
@@ -2,9 +2,7 @@ module MLS.TreeSync.ParentHash
 
 open Comparse
 open MLS.TreeSync.Types
-open MLS.TreeKEM.Types
-open MLS.TreeKEM
-open MLS.TreeSyncTreeKEMBinder
+open MLS.TreeSync.Hash
 open MLS.Crypto
 open MLS.Tree
 open MLS.NetworkTypes
@@ -15,30 +13,13 @@ open MLS.Result
 noeq type parent_hash_input_nt (bytes:Type0) {|bytes_like bytes|} = {
   public_key: hpke_public_key_nt bytes;
   parent_hash: mls_bytes bytes;
-  original_child_resolution: mls_seq bytes ps_hpke_public_key_nt;
+  original_sibling_tree_hash: mls_bytes bytes;
 }
 
 %splice [ps_parent_hash_input_nt] (gen_parser (`parent_hash_input_nt))
 
 instance parseable_serializeable_parent_hash_input_nt (bytes:Type0) {|bytes_like bytes|}: parseable_serializeable bytes (parent_hash_input_nt bytes) =
   mk_parseable_serializeable ps_parent_hash_input_nt
-
-val compute_parent_hash_treekem: #bytes:Type0 -> {|crypto_bytes bytes|} -> #l:nat -> #n:tree_size l -> hpke_public_key_nt bytes -> bytes -> treekem bytes l n -> list nat -> result (lbytes bytes (hash_length #bytes))
-let compute_parent_hash_treekem #bytes #cb #l #n public_key parent_hash sibling forbidden_leaves =
-  let original_child_resolution = original_tree_resolution forbidden_leaves sibling in
-  let original_child_resolution_nt = List.Tot.map (fun (x:hpke_public_key bytes) -> x <: hpke_public_key_nt bytes) original_child_resolution in
-  if not (length parent_hash < pow2 30) then
-    internal_failure "compute_parent_hash: parent_hash too long"
-  else if not (bytes_length ps_hpke_public_key_nt original_child_resolution_nt < pow2 30) then
-    internal_failure "compute_parent_hash: original_child_resolution too big"
-  else (
-    Seq.lemma_list_seq_bij original_child_resolution_nt;
-    hash_hash (serialize (parent_hash_input_nt bytes) ({
-      public_key = public_key;
-      parent_hash = parent_hash;
-      original_child_resolution = Seq.seq_of_list original_child_resolution_nt;
-    }))
-  )
 
 val get_public_key_from_content: #bytes:Type0 -> {|bytes_like bytes|} -> bytes -> result (hpke_public_key_nt bytes)
 let get_public_key_from_content #bytes #bl content =
@@ -47,31 +28,65 @@ let get_public_key_from_content #bytes #bl content =
     (parse (treekem_content_nt bytes) content);
   return content.public_key
 
-//TODO possible performance optimisation: no need to convert root from treesync to treekem: we only need to convert its content
-val compute_parent_hash_from_sibling: #bytes:Type0 -> {|crypto_bytes bytes|} -> #l:nat -> #ls:nat -> #n:tree_size l -> #ns:tree_size ls -> content:bytes -> parent_parent_hash:bytes -> nat -> treesync bytes l n -> nat -> treesync bytes ls ns -> result (lbytes bytes (hash_length #bytes))
-let compute_parent_hash_from_sibling #bytes #cb #l #ls #n #ns content parent_parent_hash nb_left_leaves_root root nb_left_leaves_sibling sibling =
-  root_kem <-- treesync_to_treekem_aux nb_left_leaves_root root;
-  sibling_kem <-- treesync_to_treekem_aux nb_left_leaves_sibling sibling;
-  public_key <-- get_public_key_from_content content;
-  root_kem_onp <-- (
-    match root_kem with
-    | TNode root_onp _ _ ->
-      return root_onp
-    | _ ->
-      internal_failure "compute_parent_hash_from_sibling: `root` must be an internal node"
-  );
-  let forbidden_keys =
-    match root_kem_onp with
-    | None -> []
-    | Some root_np ->
-      (root_np <: key_package bytes).unmerged_leaves
-  in
-  compute_parent_hash_treekem public_key parent_parent_hash sibling_kem forbidden_keys
+val mk_full_blank_tree: #bytes:Type0 -> {|bytes_like bytes|} -> l:nat -> treesync bytes l (pow2 l)
+let rec mk_full_blank_tree #bytes #bl l =
+  if l = 0 then
+    TLeaf None
+  else
+    TNode None (mk_full_blank_tree (l-1)) (mk_full_blank_tree (l-1))
 
-val compute_parent_hash_from_dir: #bytes:Type0 -> {|crypto_bytes bytes|} -> #l:nat -> #n:tree_size l -> content:bytes -> parent_parent_hash:bytes -> nat -> treesync bytes l n -> direction -> result (lbytes bytes (hash_length #bytes))
-let compute_parent_hash_from_dir #bytes #cb #l #n content parent_parent_hash nb_left_leaves root dir =
+val fully_extend: #bytes:Type0 -> {|bytes_like bytes|} -> #l:nat -> #n:tree_size l -> treesync bytes l n -> treesync bytes l (pow2 l)
+let rec fully_extend #bytes #bl #l #n t =
+  match t with
+  | TLeaf olp ->
+    TLeaf olp
+  | TSkip _ t' ->
+    TNode None (fully_extend t') (mk_full_blank_tree _)
+  | TNode onp left right ->
+    TNode onp left (fully_extend right)
+
+val un_add: #bytes:Type0 -> {|bytes_like bytes|} -> #l:nat -> #n:tree_size l -> treesync bytes l n -> list nat -> nat -> treesync bytes l n
+let rec un_add #bytes #bl #l #n t leaves nb_left_leaves =
+  match t with
+  | TLeaf olp -> (
+    if List.Tot.mem nb_left_leaves leaves then
+      TLeaf None
+    else
+      TLeaf olp
+  )
+  | TSkip _ t' ->
+    TSkip _ (un_add t' leaves nb_left_leaves)
+  | TNode onp left right ->
+    let new_onp =
+      match onp with
+      | None -> None
+      | Some np -> (
+        let new_unmerged_leaves = List.Tot.filter (fun l -> not (List.Tot.mem l leaves)) np.unmerged_leaves in
+        Some ({ np with unmerged_leaves = new_unmerged_leaves } <: node_package_t bytes)
+      )
+    in
+    let new_left = un_add left leaves nb_left_leaves in
+    let new_right = un_add right leaves (nb_left_leaves + pow2 (l-1)) in
+    TNode new_onp new_left new_right
+
+val compute_parent_hash_from_sibling: #bytes:Type0 -> {|crypto_bytes bytes|} -> #ls:nat -> #ns:tree_size ls -> node_package_t bytes -> nat -> treesync bytes ls ns -> result (lbytes bytes (hash_length #bytes))
+let compute_parent_hash_from_sibling #bytes #cb #ls #ns root_np nb_left_leaves_sibling sibling =
+  public_key <-- get_public_key_from_content root_np.content.content;
+  original_sibling_tree_hash <-- tree_hash (fully_extend (un_add sibling root_np.unmerged_leaves nb_left_leaves_sibling));
+  if not (length root_np.parent_hash < pow2 30) then
+    internal_failure "compute_parent_hash_from_sibling: parent_hash too long"
+  else (
+    hash_hash (serialize (parent_hash_input_nt bytes) ({
+      public_key;
+      parent_hash = root_np.parent_hash;
+      original_sibling_tree_hash;
+    }))
+  )
+
+val compute_parent_hash_from_dir: #bytes:Type0 -> {|crypto_bytes bytes|} -> #l:nat -> #n:tree_size l -> nat -> treesync bytes l n -> direction -> result (lbytes bytes (hash_length #bytes))
+let compute_parent_hash_from_dir #bytes #cb #l #n nb_left_leaves root dir =
   match root with
-  | TNode _ left right ->
+  | TNode (Some root_np) left right ->
     let (_, sibling) = order_subtrees dir (left, right) in
     let nb_left_leaves_sibling =
       if dir = Left then
@@ -79,5 +94,5 @@ let compute_parent_hash_from_dir #bytes #cb #l #n content parent_parent_hash nb_
       else
         nb_left_leaves
     in
-    compute_parent_hash_from_sibling content parent_parent_hash nb_left_leaves root nb_left_leaves_sibling sibling
-  | _ -> internal_failure "compute_parent_hash_from_dir: `root` must be an internal node"
+    compute_parent_hash_from_sibling root_np nb_left_leaves_sibling sibling
+  | _ -> internal_failure "compute_parent_hash_from_dir: `root` must be a non-blank internal node"
